src/fs/Util.fs
@@ -55,3 +55,15 @@ let slice l i j = take (remove l i) (j - i + 1)
 let rec ofInt i j =
   if j <= 0 then []
   else (i % 2 = 1)::(ofInt (i / 2) (j - 1))
+
+let rec unins l y = match l with
+  | []    -> [y]
+  | x::xs -> if x = y then x::xs else x::(unins xs y)
+
+let listUnion x y = List.fold_left unins y x
+
+let rec symins l y = match l with
+  | []    -> [y]
+  | x::xs -> if x = y then xs else x::(symins xs y)
+
+let listSymdiff x y = List.fold_left symins y x
